src/Executable_Surface/Codegen/Export/Voblint_Codegen.thy
@@ -118,7 +118,7 @@ export_code
   state_point state_context state_value state_checks state_diagnostics
   route_point route_context route_callee route_targets
   check_point check_exp check_verdict
-  global_var global_val
+  global_key global_state Global_Shared Global_Seed
   diagnostic_point diagnostic_obligation diagnostic_verdict arithmetic_operation
   Check_Proved Check_Refuted Check_Unknown
   Bot Lifted
